Support for push2 and pop4. Reader/Writer interfaces changed

src/Ring.fst
@@ -9,7 +9,7 @@ module U8 =   FStar.UInt8
 open LowStar.BufferOps
 open FStar.HyperStack.ST
 include LowStar.Monotonic.Buffer
-
+open FStar.Seq
 
 
 
@@ -54,23 +54,6 @@ let incr_ht_spec (ht:UInt32.t) (rsize:UInt32.t{ UInt32.lt ht rsize}) : GTot  (l:
   if UInt32.eq ht' rsize then 0ul
   else ht'
 
-let is_rb_full_spec (#a:eqtype) (h:HS.mem) (r:ringstruct a {well_formed_rb h r}): GTot bool
-  = 
-//  let rsize = r.rsize in
-  let head =  B.get h r.headptr 0 in
-  let tail = B.get h  r.tailptr 0 in
-  let rsize = r.rsize in
-  let head' = incr_ht_spec head rsize in  
-  head' = tail
-
-let is_rb_empty_spec (#a:eqtype) (h:HS.mem) (r:ringstruct a): GTot bool
-  = 
-//  let rsize = r.rsize in
-  let head =  B.get h r.headptr 0 in
-  let tail = B.get h  r.tailptr 0 in
-   UInt32.eq head tail
-
-
 
 
 let get_head_spec (#a:eqtype) (h:HS.mem) (r:ringstruct a {well_formed_rb h r}): GTot (r':UInt32.t {UInt32.lt r' r.rsize})
@@ -79,14 +62,122 @@ let get_head_spec (#a:eqtype) (h:HS.mem) (r:ringstruct a {well_formed_rb h r}): 
 let get_tail_spec (#a:eqtype) (h:HS.mem) (r:ringstruct a {well_formed_rb h r}): GTot (r':UInt32.t {UInt32.lt r' r.rsize})
 = B.get h r.tailptr 0
 
+//increment the head by 1 push
 let incr_head_spec (#a:eqtype) (h:HS.mem) (r:ringstruct a {well_formed_rb h r}): GTot (r':UInt32.t {UInt32.lt r' r.rsize})
  = let head = B.get h r.headptr 0 in
   incr_ht_spec head r.rsize
+
+//increment the head by 2 push
+let incr2_head_spec (#a:eqtype) (h:HS.mem) (r:ringstruct a {well_formed_rb h r /\ (UInt32.gt r.rsize 2ul)}): GTot (r':UInt32.t {UInt32.lt r' r.rsize})
+=
+let ht = B.get h r.headptr 0 in
+let rsize = r.rsize in
+let _ = assert(UInt32.lt ht rsize) in
+let ht1 = UInt32.add ht 1ul in
+  if (UInt32.eq ht1 rsize) then 1ul
+  else
+    let _ = assert(UInt32.lt ht1 rsize) in
+    let ht2 = UInt32.add ht1 1ul in
+       if (UInt32.eq ht2 rsize)  then 0ul
+         else ht2
+
+//increment the head by 3 push
+let incr3_head_spec (#a:eqtype) (h:HS.mem) (r:ringstruct a {well_formed_rb h r /\ (UInt32.gt r.rsize 3ul)}): GTot (r':UInt32.t {UInt32.lt r' r.rsize})
+=
+let ht = B.get h r.headptr 0 in
+let rsize = r.rsize in
+let _ = assert(UInt32.lt ht rsize) in
+let ht1 = UInt32.add ht 1ul in
+  if (UInt32.eq ht1 rsize) then 2ul
+  else
+    let _ = assert(UInt32.lt ht1 rsize) in
+    let ht2 = UInt32.add ht1 1ul in
+       if (UInt32.eq ht2 rsize)  then 1ul
+         else 
+           let _ = assert(UInt32.lt ht2 rsize) in
+           let ht3 = UInt32.add ht2 1ul in
+           if (UInt32.eq ht3 rsize)  then 0ul
+             else ht3
+
+//increment the head by 4 push
+let incr4_head_spec (#a:eqtype) (h:HS.mem) (r:ringstruct a {well_formed_rb h r /\ (UInt32.gt r.rsize 4ul)}): GTot (r':UInt32.t {UInt32.lt r' r.rsize})
+=
+let ht = B.get h r.headptr 0 in
+let rsize = r.rsize in
+let _ = assert(UInt32.lt ht rsize) in
+let ht1 = UInt32.add ht 1ul in
+  if (UInt32.eq ht1 rsize) then 3ul
+  else
+    let _ = assert(UInt32.lt ht1 rsize) in
+    let ht2 = UInt32.add ht1 1ul in
+       if (UInt32.eq ht2 rsize)  then 2ul
+         else 
+           let _ = assert(UInt32.lt ht2 rsize) in
+           let ht3 = UInt32.add ht2 1ul in
+           if (UInt32.eq ht3 rsize)  then 1ul
+             else 
+               let _ = assert(UInt32.lt ht3 rsize) in
+               let ht4 = UInt32.add ht3 1ul in
+               if (UInt32.eq ht4 rsize) then 0ul
+               else ht4
   
+
 let incr_tail_spec (#a:eqtype) (h:HS.mem) (r:ringstruct a {well_formed_rb h r}): GTot (r':UInt32.t {UInt32.lt r' r.rsize})
   = let tail = B.get h r.tailptr 0 in
   incr_ht_spec tail r.rsize
+
+let incr2_tail_spec (#a:eqtype) (h:HS.mem) (r:ringstruct a {well_formed_rb h r /\ (UInt32.gt r.rsize 2ul)}): GTot (r':UInt32.t {UInt32.lt r' r.rsize})
+=
+let ht = B.get h r.tailptr 0 in
+let rsize = r.rsize in
+let _ = assert(UInt32.lt ht rsize) in
+let ht1 = UInt32.add ht 1ul in
+  if (UInt32.eq ht1 rsize) then 1ul
+  else
+    let _ = assert(UInt32.lt ht1 rsize) in
+    let ht2 = UInt32.add ht1 1ul in
+       if (UInt32.eq ht2 rsize)  then 0ul
+         else ht2
+
+let incr3_tail_spec (#a:eqtype) (h:HS.mem) (r:ringstruct a {well_formed_rb h r /\ (UInt32.gt r.rsize 3ul)}): GTot (r':UInt32.t {UInt32.lt r' r.rsize})
+=
+let ht = B.get h r.tailptr 0 in
+let rsize = r.rsize in
+let _ = assert(UInt32.lt ht rsize) in
+let ht1 = UInt32.add ht 1ul in
+  if (UInt32.eq ht1 rsize) then 2ul
+  else
+    let _ = assert(UInt32.lt ht1 rsize) in
+    let ht2 = UInt32.add ht1 1ul in
+       if (UInt32.eq ht2 rsize)  then 1ul
+         else 
+           let _ = assert(UInt32.lt ht2 rsize) in
+           let ht3 = UInt32.add ht2 1ul in
+           if (UInt32.eq ht3 rsize)  then 0ul
+             else ht3
+
+let incr4_tail_spec (#a:eqtype) (h:HS.mem) (r:ringstruct a {well_formed_rb h r /\ (UInt32.gt r.rsize 4ul)}): GTot (r':UInt32.t {UInt32.lt r' r.rsize})
+=
+let ht = B.get h r.tailptr 0 in
+let rsize = r.rsize in
+let _ = assert(UInt32.lt ht rsize) in
+let ht1 = UInt32.add ht 1ul in
+  if (UInt32.eq ht1 rsize) then 3ul
+  else
+    let _ = assert(UInt32.lt ht1 rsize) in
+    let ht2 = UInt32.add ht1 1ul in
+       if (UInt32.eq ht2 rsize)  then 2ul
+         else 
+           let _ = assert(UInt32.lt ht2 rsize) in
+           let ht3 = UInt32.add ht2 1ul in
+           if (UInt32.eq ht3 rsize)  then 1ul
+             else 
+               let _ = assert(UInt32.lt ht3 rsize) in
+               let ht4 = UInt32.add ht3 1ul in
+               if (UInt32.eq ht4 rsize) then 0ul
+               else ht4
   
+
 let tail_unmodified_spec (#a:eqtype) (h0:HS.mem) (h1:HS.mem) (r0:ringstruct a) (r1: ringstruct a) : GTot bool
  = UInt32.eq (B.get h0 r0.tailptr 0) (B.get h1 r1.tailptr 0) 
 
@@ -97,14 +188,94 @@ let rsize_unmodified_spec (#a:eqtype) (r0:ringstruct a) (r1: ringstruct a) : GTo
  = UInt32.eq r0.rsize r1.rsize 
 
 let incr_ht (ht:UInt32.t) (rsize:UInt32.t{UInt32.lt ht rsize}) : Tot  (i:UInt32.t {UInt32.lt i rsize})
-//(requires UInt32.lt ht rsize)
-//(ensures fun i -> UInt32.lt i rsize)
   // increment by 1 and check if the buffer is full
   // if so, reset it
  = let ht' = UInt32.add ht 1ul in
   if UInt32.eq ht' rsize then 0ul
   else ht'
 
+
+
+let get_current_size (head:UInt32.t) (tail:UInt32.t) (rsize:UInt32.t{UInt32.lt head rsize /\ UInt32.lt tail rsize}) : Tot  (i:UInt32.t {UInt32.lte i rsize})
+ =
+  (*
+   *  ----------------------
+   *  |  |  |  |  |  |  |  | 
+   *  ----------------------
+   *   t        h
+   *  ----------------------
+   *  |  |  |  |  |  |  |  | 
+   *  ----------------------
+   *      h     t
+   *)
+   if (UInt32.gte head  tail) then (UInt32.sub head tail)
+   else //  (UInt32.lt head  tail)
+   (UInt32.sub rsize (UInt32.sub tail head))
+   
+
+let get_remaining_space (head:UInt32.t) (tail:UInt32.t) (rsize:UInt32.t{UInt32.lt head rsize /\ UInt32.lt tail rsize}) : Tot  (i:UInt32.t {UInt32.lte i rsize})
+ =
+  (*
+   *  ----------------------
+   *  |  |  |  |  |  |  |  | 
+   *  ----------------------
+   *   t        h
+   *  ----------------------
+   *  |  |  |  |  |  |  |  | 
+   *  ----------------------
+   *      h     t
+   *)
+   let c = get_current_size head tail rsize in
+     (UInt32.sub rsize c)
+   
+let get_current_size_spec (#a:eqtype) (h:HS.mem) (r:ringstruct a {well_formed_rb h r}) : GTot (i:UInt32.t {UInt32.lte i r.rsize})
+= 
+let head = B.get h r.headptr 0 in
+let tail = B.get h r.tailptr 0 in
+let rsize = r.rsize in
+get_current_size head tail rsize
+
+
+let remaining_space_spec (#a:eqtype) (h:HS.mem) (r:ringstruct a{well_formed_rb h r}): GTot  (r':UInt32.t {UInt32.lte r' r.rsize})
+ =
+  let head = B.get h r.headptr 0 in
+  let tail = B.get h  r.tailptr 0 in
+  let rsize = r.rsize in
+  (*
+   *  ----------------------
+   *  |  |  |  |  |  |  |  | 
+   *  ----------------------
+   *   t        h
+   *)
+   let c = get_current_size head tail rsize in
+     (UInt32.sub rsize c)
+   
+
+let is_rb_full_spec (#a:eqtype) (h:HS.mem) (r:ringstruct a {well_formed_rb h r}): GTot bool
+  = let sz = get_current_size_spec h r in
+  (UInt32.eq sz (UInt32.sub r.rsize 1ul))
+
+let is_rb_empty_spec (#a:eqtype) (h:HS.mem) (r:ringstruct a {well_formed_rb h r}): GTot bool
+  = let sz = get_current_size_spec h r in
+  (UInt32.eq sz 0ul)
+
+
+let is_poppable (#a:eqtype) (r:ringstruct a): ST bool
+(requires fun h -> live_rb h r
+                /\ well_formed_rb h r
+)
+(ensures fun h0 s h1 -> live_rb h1 r
+                     /\ well_formed_rb h1 r
+                     /\ modifies loc_none h0 h1
+                     /\ ((s == true) ==>  not (is_rb_empty_spec h1 r))
+)
+= let head = !* r.headptr in
+let tail = !* r.tailptr in
+let rsize = r.rsize in
+let space = get_current_size head tail rsize in
+if (UInt32.gt space 0ul) then true
+else false
+                
 
 (* push: pushes an element at the head position
  * The pre-condition says that the invariants of the ringbuffer, namely,
@@ -135,17 +306,59 @@ let push (#a:eqtype) (r: ringstruct a) (v: a) : ST unit
                       /\ not (is_rb_empty_spec h1 r)
                     )
   =
-(* 
-  let tail = !* r.tailptr in
-  let b = is_rb_full rsize head tail in
-  if (not b) then
- *)   // update the buffer at head and then
+   // update the buffer at head and then
     // increment the head
   let rsize = r.rsize in
   let head =  !* r.headptr in
   let _ =  r.headptr *= (incr_ht head rsize) in
   B.upd r.rbuf head v
-     
+
+let push2 (#a:eqtype) (r: ringstruct a) (v1:a) (v2:a) : ST unit
+  (requires fun h -> live_rb h r
+                  /\  well_formed_rb h r
+//                  /\ not (is_rb_full_spec h r)
+                     /\ UInt32.gt (remaining_space_spec h r) 4ul
+                     /\ (UInt32.gt r.rsize 4ul)
+                   )
+  (ensures fun h0 _ h1 -> 
+                    live_rb h1 r 
+                    /\ modifies (loc_union (loc_buffer r.rbuf)  (loc_buffer r.headptr)) h0 h1
+                    /\ tail_unmodified_spec h0 h1 r r 
+                    /\ well_formed_rb h1 r
+                    /\ as_seq h1 r.rbuf == (Seq.upd (Seq.upd (as_seq h0 r.rbuf) (UInt32.v (get_head_spec h0 r)) v1)  (UInt32.v (incr_head_spec h0 r)) v2)
+                    /\  get_head_spec h1 r == incr2_head_spec h0 r
+//                    /\ not (is_rb_empty_spec h1 r)
+                    )
+  =
+  push r v1;
+  push r v2
+
+(*
+SMT timing out. Fix this later
+let push4 (#a:eqtype) (r: ringstruct a) (v1:a) (v2:a) (v3:a) (v4:a) : ST unit
+  (requires fun h -> live_rb h r
+                  /\  well_formed_rb h r
+//                  /\ not (is_rb_full_spec h r)
+                     /\ UInt32.gt (remaining_space_spec h r) 4ul
+                     /\ (UInt32.gt r.rsize 4ul)
+                   )
+  (ensures fun h0 _ h1 -> 
+                    live_rb h1 r 
+                    /\ modifies (loc_union (loc_buffer r.rbuf)  (loc_buffer r.headptr)) h0 h1
+                    /\ tail_unmodified_spec h0 h1 r r 
+                    /\ well_formed_rb h1 r
+                    /\ as_seq h1 r.rbuf == (Seq.upd (Seq.upd (Seq.upd (Seq.upd (as_seq h0 r.rbuf) (UInt32.v (get_head_spec h0 r)) v1)  (UInt32.v (incr_head_spec h0 r)) v2)  (UInt32.v (incr2_head_spec h0 r)) v3)  (UInt32.v (incr3_head_spec h0 r)) v4)
+//                    /\ as_seq h1 r.rbuf == (Seq.upd (Seq.upd (Seq.upd (as_seq h0 r.rbuf) (UInt32.v (get_head_spec h0 r)) v1)  (UInt32.v (incr_head_spec h0 r)) v2)  (UInt32.v (incr2_head_spec h0 r)) v3)
+                    /\  get_head_spec h1 r == incr4_head_spec h0 r
+//                    /\ not (is_rb_empty_spec h1 r)
+                    )
+  =
+  push r v1;
+  push r v2;
+  push r v3;
+  push r v4
+
+*)
 noeq
 type option 'a =
  | Error : option 'a
@@ -161,7 +374,8 @@ type option 'a =
 let pop (#a:eqtype) (r: ringstruct a) : ST a 
   (requires fun h0 -> live_rb h0 r 
                      /\ well_formed_rb h0 r
-                     /\ not (is_rb_empty_spec h0 r)
+//                     /\ not (is_rb_empty_spec h0 r)
+                     /\ (UInt32.gt (get_current_size_spec h0 r) 0ul)
                     )
   (ensures fun h0 v h1 -> live_rb h1 r
                    /\ well_formed_rb h1 r
@@ -170,20 +384,45 @@ let pop (#a:eqtype) (r: ringstruct a) : ST a
                    /\ head_unmodified_spec h0 h1 r r 
                    /\ (v == Seq.index (as_seq h1 r.rbuf) (UInt32.v (get_tail_spec h0 r)))
                    /\ (get_tail_spec h1 r == incr_tail_spec h0 r)
+                   /\ (get_current_size_spec h1 r) = UInt32.sub (get_current_size_spec h0 r) 1ul
+//                   /\ UInt32.lte (get_current_size_spec h1 r)  (get_current_size_spec h0 r)
   )
   = 
   let rsize = r.rsize in
-  let head =  !* r.headptr in
   let tail = !* r.tailptr in
-  let b = is_rb_empty rsize head tail in
-  if (not b) then
-    // First deref the buffer and then increment the tail
-    let v = B.index r.rbuf tail  in
-    let _ = r.tailptr *=  incr_ht tail rsize in
-    v
-  
+//  let head = !* r.headptr in
+  // First deref the buffer and then increment the tail
+  let _ = r.tailptr *=  (incr_ht tail rsize) in
+  B.index r.rbuf tail
 
 
+
+//Handy routines
+// Return a sequence of bytes
+let pop4 (#a:eqtype) (r: ringstruct a) : ST (a*a*a*a) 
+  (requires fun h0 -> live_rb h0 r 
+                     /\ well_formed_rb h0 r
+                     /\ UInt32.gt (get_current_size_spec h0 r) 4ul
+                     /\ (UInt32.gt r.rsize 4ul)
+                    )
+  (ensures fun h0 (v1, v2, v3, v4) h1 -> live_rb h1 r
+                   /\ well_formed_rb h1 r
+                   /\ modifies (loc_buffer r.tailptr) h0 h1
+                   /\ as_seq h1 r.rbuf == as_seq h0 r.rbuf
+                   /\ head_unmodified_spec h0 h1 r r 
+                   /\ (v1 == Seq.index (as_seq h1 r.rbuf) (UInt32.v (get_tail_spec h0 r)))
+                   /\ (v2 == Seq.index (as_seq h1 r.rbuf) (UInt32.v (incr_tail_spec h0 r)))
+                   /\ (v3 == Seq.index (as_seq h1 r.rbuf) (UInt32.v (incr2_tail_spec h0 r)))
+                   /\ (v4 == Seq.index (as_seq h1 r.rbuf) (UInt32.v (incr3_tail_spec h0 r)))
+                   /\ (get_tail_spec h1 r == incr4_tail_spec h0 r)
+  )
+  = 
+   let m1 = pop r in
+   let m2 = pop r in
+   let m3 = pop r in
+   let m4 = pop r in
+   (m1, m2, m3, m4)
+   
 // The way the fullness of ringbuffer is checked requires that the minimum size is 2
 let init (#a:eqtype) (i: a) (s:UInt32.t {UInt32.gt s 1ul}) (hid: HS.rid) : ST (ringstruct a)
 (requires fun h -> true
@@ -230,6 +469,9 @@ let rlen = 32ul in
   let _ = pop rb in  
   let _ = push rb 4uy in
   let v = pop rb in
+  push2 rb 5uy 6uy;
+//  push2 rb 7uy 8uy;
+//  let (v1, v2, v3, v4) = pop4 rb in
   v
 
    
